AwsCryptographicMaterialProviders/dafny/AwsCryptographicMaterialProviders/src/Keyrings/AwsKms/AwsKmsRsaKeyring.dfy
@@ -185,7 +185,24 @@ module AwsKmsRsaKeyring {
       return Success(Types.OnEncryptOutput(materials := returnMaterials));
     }
 
-    predicate OnDecryptEnsuresPublicly ( input: Types.OnDecryptInput , output: Result<Types.OnDecryptOutput, Types.Error> ) {true}
+    predicate OnDecryptEnsuresPublicly ( input: Types.OnDecryptInput , output: Result<Types.OnDecryptOutput, Types.Error> )
+      : (outcome: bool)
+      ensures
+        outcome ==>
+          output.Success?
+          ==>
+            && Materials.DecryptionMaterialsTransitionIsValid(
+              input.materials,
+              output.value.materials
+            )
+    {
+      output.Success?
+      ==>
+        && Materials.DecryptionMaterialsTransitionIsValid(
+          input.materials,
+          output.value.materials
+        )
+    }
 
     method OnDecrypt'(input: Types.OnDecryptInput)
       returns (res: Result<Types.OnDecryptOutput, Types.Error>)
